Impl/SuccModel.i.dfy
@@ -4,7 +4,6 @@
 include "BookkeepingModel.i.dfy"
 include "../lib/Base/Option.s.dfy"
 include "../lib/Base/Sets.i.dfy"
-include "../PivotBetree/PivotBetreeSpec.i.dfy"
 include "BucketSuccessorLoopModel.i.dfy"
 
 // See dependency graph in MainHandlers.dfy
@@ -28,10 +27,9 @@ module SuccModel {
   import opened Bounds
 
   import opened BoundedPivotsLib
+  import opened TranslationLib
   import opened Lexicographic_Byte_Order
   import BucketSuccessorLoopModel
-
-  import PBS = PivotBetreeSpec`Internal
 
   // Awkwardly split up for verification time reasons
 
@@ -40,8 +38,10 @@ module SuccModel {
       io: IO,
       key: Key,
       acc: seq<Bucket>,
+      tt: TranslationTable,
       start: UI.RangeStart,
       upTo: Option<Key>,
+      pset: Option<PrefixSet>,
       maxToFind: int,
       ref: BT.G.Reference,
       counter: uint64,
@@ -57,41 +57,63 @@ module SuccModel {
   requires maxToFind >= 1
   requires BoundedKey(node.pivotTable, key)
   requires forall i | 0 <= i < |acc| :: WFBucket(acc[i])
+  requires |acc| == 0 ==> |tt| == 0 && pset == None
+  requires |acc| > 0 ==> |tt| + 1 == |acc|
+  requires var startKey := if start.NegativeInf? then [] else start.key;
+    && (forall i | 0 <= i < |tt| :: 
+        (tt[i].Some? ==> IsPrefix(tt[i].value.newPrefix, startKey)))
+    && (pset.Some? ==> IsPrefix(pset.value.prefix, key))
+    && startKey == ApplyPrefixSet(pset, key)
   ensures var (s', io, sr) := res;
     && s'.Ready?
     && s'.cache == s.cache
   decreases counter, 0
   {
+    var startKey := if start.NegativeInf? then [] else start.key;
+
     var r := Route(node.pivotTable, key);
     var bucket := node.buckets[r];
     var acc' := acc + [bucket];
+    var tt' := if |acc| == 0 then tt else tt + [pset];
 
-    var pivot := node.pivotTable[r+1];
-    var upTo' := 
-      if pivot.Max_Element?
-      then (
-        upTo
+    var upper := 
+      if pset.None? then (
+        node.pivotTable[r+1]
       ) else (
-        var ub := GetKey(node.pivotTable, r+1);
-        if upTo.Some?
-        then (
-          var k: Key := if lt(upTo.value, ub) then upTo.value else ub;
-          Some(k)
-        ) else (
-          Some(ub)
-        )
+        var (_, right) := TranslatePivotPairInternal(KeyToElement(key), node.pivotTable[r+1], pset.value.prefix, pset.value.newPrefix);
+        right
       );
+
+    var upTo' := 
+      if upper.Max_Element? then upTo 
+      else (
+        var ub : Key := upper.e;
+        if upTo.None? then (
+          Some(ub)
+        ) else (
+          var k: Key := if lt(upTo.value, upper.e) then upTo.value else ub;
+          Some(k)
+        ));
 
     if node.children.Some? then (
       if counter == 0 then (
         (s, io, None)
       ) else (
+        var translate := Translate(node.pivotTable, node.edgeTable, key);
+        var key' := ApplyPrefixSet(translate, key);
+
+        assert translate.Some? ==> IsPrefix(translate.value.prefix, key);
+        assert pset.Some? ==> IsPrefix(pset.value.prefix, key);
+
+        var pset' := ComposePrefixSet(pset, translate);
+        ComposePrefixSetCorrect(pset, translate, pset', startKey, key, key');
+
         lemmaChildInGraph(s, ref, node.children.value[r]);
-        getPath(s, io, key, acc', start, upTo', maxToFind, node.children.value[r], counter - 1)
+        getPath(s, io, key', acc', tt', start, upTo', pset', maxToFind, node.children.value[r], counter - 1)
       )
     ) else (
       var res :=
-          BucketSuccessorLoopModel.GetSuccessorInBucketStack(acc', maxToFind, start, upTo');
+          BucketSuccessorLoopModel.GetSuccessorInBucketStack(acc', tt', maxToFind, start, upTo');
       (s, io, Some(res))
     )
   }
@@ -101,8 +123,10 @@ module SuccModel {
       io: IO,
       key: Key,
       acc: seq<Bucket>,
+      tt: TranslationTable,
       start: UI.RangeStart,
       upTo: Option<Key>,
+      pset: Option<PrefixSet>,
       maxToFind: int,
       ref: BT.G.Reference,
       counter: uint64)
@@ -113,6 +137,13 @@ module SuccModel {
   requires maxToFind >= 1
   requires ref in s.ephemeralIndirectionTable.graph
   requires forall i | 0 <= i < |acc| :: WFBucket(acc[i])
+  requires |acc| == 0 ==> |tt| == 0 && pset == None
+  requires |acc| > 0 ==> |tt| + 1 == |acc|
+  requires var startKey := if start.NegativeInf? then [] else start.key;
+    && (forall i | 0 <= i < |tt| :: 
+        (tt[i].Some? ==> IsPrefix(tt[i].value.newPrefix, startKey)))
+    && (pset.Some? ==> IsPrefix(pset.value.prefix, key))
+    && startKey == ApplyPrefixSet(pset, key)
   ensures var (s', io, sr) := res;
     && s'.Ready?
     && s'.cache == s.cache
@@ -120,8 +151,8 @@ module SuccModel {
   {
     if ref in s.cache then (
       var node := s.cache[ref];
-      if BoundedKey(node.pivotTable, key) then ( 
-        var (s0, io', pr) := getPathInternal(s, io, key, acc, start, upTo, maxToFind, ref, counter, node);
+      if BoundedKey(node.pivotTable, key) then (
+        var (s0, io', pr) := getPathInternal(s, io, key, acc, tt, start, upTo, pset, maxToFind, ref, counter, node);
         var s' := s0;
         // LruModel.LruUse(s0.lru, ref);
         // var s' := s0.(lru := LruModel.Use(s0.lru, ref));
@@ -140,50 +171,52 @@ module SuccModel {
     )
   }
 
-  function {:opaque} doSucc(s: BBC.Variables, io: IO, start: UI.RangeStart, maxToFind: int)
-  : (res : (BBC.Variables, IO, Option<UI.SuccResultList>))
-  requires BBC.Inv(s)
-  requires io.IOInit?
-  requires s.Ready?
-  requires maxToFind >= 1
-  {
-    var startKey := if start.NegativeInf? then [] else start.key;
-    getPath(s, io, startKey, [], start, None, maxToFind, BT.G.Root(), 40)
-  }
+  // function {:opaque} doSucc(s: BBC.Variables, io: IO, start: UI.RangeStart, maxToFind: int)
+  // : (res : (BBC.Variables, IO, Option<UI.SuccResultList>))
+  // requires BBC.Inv(s)
+  // requires io.IOInit?
+  // requires s.Ready?
+  // requires maxToFind >= 1
+  // {
+  //   var startKey := if start.NegativeInf? then [] else start.key;
+  //   getPath(s, io, startKey, [], [], start, None, None, maxToFind, BT.G.Root(), 40)
+  // }
 
-  predicate LookupBucketsProps(lookup: PBS.Lookup, buckets: seq<Bucket>, upTo: Option<Key>, startKey: Key)
+  predicate LookupBucketsProps(lookup: BT.Lookup, buckets: seq<Bucket>, tt: TranslationTable, upTo: Option<Key>, startKey: Key)
   {
-    && PBS.WFLookupForKey(lookup, startKey)
-    && upTo == PBS.LookupUpperBound(lookup, startKey)
-    && Last(lookup).node.children.None?
+    && BT.WFLookupForKey(lookup, startKey)
+    && BT.ValidTranslationTable(lookup, tt, 0)
+    && upTo == BT.LookupUpperBound(lookup, tt)
+    && tt == BT.LookupTranslationTable(lookup, 0, None)
+    && Last(lookup).readOp.node.children.None?
     && |lookup| == |buckets|
-    && (forall i | 0 <= i < |lookup| :: BoundedKey(lookup[i].node.pivotTable, startKey))
-    && (forall i | 0 <= i < |lookup| :: buckets[i] == lookup[i].node.buckets[Route(lookup[i].node.pivotTable, startKey)])
+    && (forall i | 0 <= i < |lookup| :: BoundedKey(lookup[i].readOp.node.pivotTable, lookup[i].currentKey))
+    && (forall i | 0 <= i < |lookup| :: buckets[i] == lookup[i].readOp.node.buckets[Route(lookup[i].readOp.node.pivotTable, lookup[i].currentKey)])
   }
 
-  lemma SatisfiesSuccBetreeStep(s: BBC.Variables, io: IO, start: UI.RangeStart,
-      res: UI.SuccResultList, buckets: seq<Bucket>, lookup: PBS.Lookup, maxToFind: int, startKey: Key, upTo: Option<Key>)
+  lemma SatisfiesSuccBetreeStep(s: BBC.Variables, io: IO, start: UI.RangeStart, res: UI.SuccResultList,
+    buckets: seq<Bucket>, tt: TranslationTable, lookup: BT.Lookup, maxToFind: int, startKey: Key, upTo: Option<Key>)
   requires BBC.Inv(s) && s.Ready?
   requires io.IOInit?
   requires maxToFind >= 1
-  requires LookupBucketsProps(lookup, buckets, upTo, startKey);
-  requires forall i | 0 <= i < |lookup| :: lookup[i].ref in s.ephemeralIndirectionTable.graph
-  requires forall i | 0 <= i < |lookup| :: MapsTo(s.cache, lookup[i].ref, lookup[i].node)
+  requires LookupBucketsProps(lookup, buckets, tt, upTo, startKey);
+  requires forall i | 0 <= i < |lookup| :: lookup[i].readOp.ref in s.ephemeralIndirectionTable.graph
+  requires forall i | 0 <= i < |lookup| :: MapsTo(s.cache, lookup[i].readOp.ref, lookup[i].readOp.node)
   requires (upTo.Some? ==> lt(startKey, upTo.value))
   requires startKey == (if start.NegativeInf? then [] else start.key)
   requires res == 
-     BucketSuccessorLoopModel.GetSuccessorInBucketStack(buckets, maxToFind, start, upTo);
-
+     BucketSuccessorLoopModel.GetSuccessorInBucketStack(buckets, tt, maxToFind, start, upTo);
   ensures ValidDiskOp(diskOp(io))
   ensures BBC.Next(s, s,
       IDiskOp(diskOp(io)).bdop,
       AdvanceOp(UI.SuccOp(start, res.results, res.end), false));
   {
     if (BucketListWellMarshalled(buckets)) {
-      BucketSuccessorLoopModel.GetSuccessorInBucketStackResult(buckets, maxToFind, start, upTo);
+      BucketSuccessorLoopModel.GetSuccessorInBucketStackResult(buckets, tt, maxToFind, start, upTo);
+      assert BT.TranslateSuccBuckets(buckets, tt, 0) == BucketSuccessorLoopModel.BGM.SuccBucketList(buckets, tt);
     }
 
-    var succStep := BT.SuccQuery(start, res.results, res.end, buckets, lookup);
+    var succStep := BT.SuccQuery(start, res.results, res.end, buckets, tt, lookup);
     assert BT.ValidSuccQuery(succStep);
     var step := BT.BetreeSuccQuery(succStep);
 
@@ -196,25 +229,116 @@ module SuccModel {
       step);
   }
 
-  lemma lemmaGetPathResult(s: BBC.Variables, io: IO, startKey: Key, acc: seq<Bucket>, lookup: PBS.Lookup, start: UI.RangeStart, upTo: Option<Key>, maxToFind: int, ref: BT.G.Reference, counter: uint64)
+  function NextPrefixSet(lookup: BT.Lookup, tt: TranslationTable): (pset: Option<PrefixSet>)
+  requires |lookup| > 0
+  requires BT.LookupTranslationTable.requires(lookup, 0, None)
+  requires tt == BT.LookupTranslationTable(lookup, 0, None)
+  {
+    var node := Last(lookup).readOp.node;
+    var curr := Translate(node.pivotTable, node.edgeTable, Last(lookup).currentKey);
+    var prev := if |tt| == 0 then None else Last(tt);
+
+    assert curr.Some? ==> IsPrefix(curr.value.prefix, Last(lookup).currentKey);
+    assert prev.Some? ==> IsPrefix(prev.value.prefix, Last(lookup).currentKey);
+    ComposePrefixSet(prev, curr)
+  }
+
+  lemma TranslationTableEquivIter(lookup: BT.Lookup, tt: TranslationTable, idx: int, prev: Option<PrefixSet>)
+  requires 0 <= idx < |tt|
+  requires |lookup| > 2 && |tt| > 1
+  requires |tt| + 1  == |lookup|
+  requires idx == 0 ==> prev.None?
+  requires idx > 0 ==> prev == tt[idx-1]
+  requires BT.LookupVisitsWFNodes(lookup)
+  requires BT.LookupBoundedKey(lookup)
+  requires BT.LookupFollowsChildEdges(lookup)
+  requires BT.LookupFollowsChildEdges(lookup[..|lookup|-1])
+  requires prev.Some? ==> IsPrefix(prev.value.prefix, lookup[idx].currentKey)
+  requires lookup[0].currentKey == ApplyPrefixSet(prev, lookup[idx].currentKey)
+  requires tt[..|tt|-1] == BT.LookupTranslationTable(lookup[..|lookup|-1], 0, None)
+  requires tt[|tt|-1] == NextPrefixSet(lookup[..|lookup|-1], tt[..|tt|-1])
+  requires tt[idx..|tt|-1] == BT.LookupTranslationTable(lookup[..|lookup|-1], idx, prev)
+  decreases |lookup| - idx
+  ensures tt[idx..] == BT.LookupTranslationTable(lookup, idx, prev)
+  {
+    var tt' := BT.LookupTranslationTable(lookup, idx, prev);
+
+    if idx == |lookup|-2 {
+      assert tt' == [ NextPrefixSet(lookup[..|lookup|-1], tt[..|tt|-1]) ] by {
+       BT.reveal_LookupTranslationTable();
+      }
+    } else {
+      assert idx < |lookup|-2;
+      assert 0 <= idx+1 < |tt|;
+  
+      assert tt[idx] == tt[..|tt|-1][idx];
+      assert lookup[idx+1] == lookup[..|lookup|-1][idx+1];      
+
+      assert tt[idx].Some? ==> IsPrefix(tt[idx].value.prefix, lookup[idx+1].currentKey);
+      assert lookup[0].currentKey == ApplyPrefixSet(tt[idx], lookup[idx+1].currentKey);
+
+      TranslationTableEquivIter(lookup, tt, idx+1, tt[idx]);
+      assert tt[idx+1..] == BT.LookupTranslationTable(lookup, idx+1, tt[idx]);
+
+      assert lookup[idx] == lookup[..|lookup|-1][idx];
+      assert idx == 0 ==> prev.None?;
+      assert idx > 0 ==> (tt[idx-1] == tt[..|tt|-1][idx-1]);
+
+      assert tt'[0] == tt[idx] by { BT.reveal_LookupTranslationTable(); }
+      assert tt[idx..] == tt';
+    }
+  }
+
+  lemma TranslationTableEquiv(lookup: BT.Lookup, tt: TranslationTable)
+  requires |lookup| > 1 && |tt| > 0
+  requires BT.LookupVisitsWFNodes(lookup)
+  requires BT.LookupBoundedKey(lookup)
+  requires BT.LookupFollowsChildEdges(lookup)
+  requires BT.LookupFollowsChildEdges(lookup[..|lookup|-1])
+  requires tt[..|tt|-1] == BT.LookupTranslationTable(lookup[..|lookup|-1], 0, None)
+  requires tt[|tt|-1] == NextPrefixSet(lookup[..|lookup|-1], tt[..|tt|-1])
+  ensures tt == BT.LookupTranslationTable(lookup, 0, None)
+  {
+    BT.reveal_LookupTranslationTable();
+    if |lookup| == 2 {
+    } else {
+      TranslationTableEquivIter(lookup, tt, 0, None);
+    }
+  }
+
+  lemma lemmaGetPathResult(s: BBC.Variables, io: IO, startKey: Key, key: Key, acc: seq<Bucket>, tt: TranslationTable,
+    lookup: BT.Lookup, start: UI.RangeStart, upTo: Option<Key>, pset: Option<PrefixSet>, maxToFind: int, ref: BT.G.Reference, counter: uint64)
   requires BBC.Inv(s) && s.Ready?
   requires io.IOInit?
   requires maxToFind >= 1
   requires forall i | 0 <= i < |acc| :: WFBucket(acc[i])
   requires ref in s.ephemeralIndirectionTable.graph
-  requires |lookup| > 0 ==> PBS.WFLookupForKey(lookup, startKey)
-  requires |lookup| > 0 ==> Last(lookup).node.children.Some?
-  requires |lookup| > 0 ==> ref == Last(lookup).node.children.value[Route(Last(lookup).node.pivotTable, startKey)]
+  requires |lookup| > 0 ==> BT.WFLookupForKey(lookup, startKey)
+  requires |lookup| > 0 ==> Last(lookup).readOp.node.children.Some?
+  requires |lookup| > 0 ==> tt == BT.LookupTranslationTable(lookup, 0, None)
+  requires |lookup| > 0 ==> upTo == BT.LookupUpperBound(lookup, tt)
+  requires |lookup| > 0 ==> key == TranslateKey(Last(lookup).readOp.node.pivotTable, Last(lookup).readOp.node.edgeTable, Last(lookup).currentKey)
+  requires |lookup| > 0 ==> ref == Last(lookup).readOp.node.children.value[Route(Last(lookup).readOp.node.pivotTable, Last(lookup).currentKey)]
+  requires |lookup| > 0 ==> pset == NextPrefixSet(lookup, tt)
+
   requires |lookup| == 0 ==> ref == BT.G.Root()
-  requires upTo == PBS.LookupUpperBound(lookup, startKey)
+  requires |lookup| == 0 ==> key == startKey
+  requires |lookup| == 0 ==> |tt| == 0 && pset == None
+  requires |lookup| == 0 ==> upTo.None?
   requires |lookup| == |acc|
-  requires forall i | 0 <= i < |lookup| :: acc[i] == lookup[i].node.buckets[Route(lookup[i].node.pivotTable, startKey)]
-  requires (forall i | 0 <= i < |lookup| :: lookup[i].ref in s.ephemeralIndirectionTable.graph)
-  requires forall i | 0 <= i < |lookup| :: lookup[i].ref in s.cache && lookup[i].node == s.cache[lookup[i].ref]
+
+  requires forall i | 0 <= i < |tt| :: (tt[i].Some? ==> IsPrefix(tt[i].value.newPrefix, startKey))
+  requires pset.Some? ==> IsPrefix(pset.value.prefix, key)
+  requires startKey == ApplyPrefixSet(pset, key)
+
+  requires forall i | 0 <= i < |lookup| :: acc[i] == lookup[i].readOp.node.buckets[Route(lookup[i].readOp.node.pivotTable, lookup[i].currentKey)]
+  requires forall i | 0 <= i < |lookup| :: lookup[i].readOp.ref in s.ephemeralIndirectionTable.graph
+  requires forall i | 0 <= i < |lookup| :: lookup[i].readOp.ref in s.cache && lookup[i].readOp.node == s.cache[lookup[i].readOp.ref]
   requires upTo.Some? ==> lt(startKey, upTo.value)
   requires startKey == (if start.NegativeInf? then [] else start.key)
   decreases counter
-  ensures var (s', io', res) := getPath(s, io, startKey, acc, start, upTo, maxToFind, ref, counter);
+
+  ensures var (s', io', res) := getPath(s, io, key, acc, tt, start, upTo, pset, maxToFind, ref, counter);
       && ValidDiskOp(diskOp(io'))
       && IDiskOp(diskOp(io')).jdop.NoDiskOp?
       && (res.Some? ==> BBC.Next(s, s',
@@ -234,57 +358,86 @@ module SuccModel {
       ) */
   {
     reveal_getPath();
-    reveal_getPathInternal();
-
     if ref in s.cache {
       var node := s.cache[ref];
-      if BoundedKey(node.pivotTable, startKey) {
-        var r := Route(node.pivotTable, startKey);
-        var bucket := node.buckets[r];
-        var acc1 := acc + [bucket];
-        var lookup1 := lookup + [BT.G.ReadOp(ref, node)];
+      if BoundedKey(node.pivotTable, key) {
+        reveal_getPathInternal();
 
-        forall idx | PBS.ValidLayerIndex(lookup1, idx) && idx < |lookup1| - 1
-        ensures PBS.LookupFollowsChildRefAtLayer(startKey, lookup1, idx)
+        var r := Route(node.pivotTable, key);
+        var bucket := node.buckets[r];
+        var acc' := acc + [bucket];
+        var tt' := if |acc| == 0 then tt else tt + [pset];
+
+        var lookup' := lookup + [ BT.Layer(BT.G.ReadOp(ref, node), key) ];
+
+        forall idx | BT.ValidLayerIndex(lookup', idx) && idx < |lookup'| - 1
+        ensures BT.LookupFollowsChildRefAtLayer(lookup', idx)
+        ensures BT.LookupFollowsChildEdgeAtLayer(lookup', idx)
         {
-          if idx == |lookup1| - 2 {
-            assert PBS.LookupFollowsChildRefAtLayer(startKey, lookup1, idx);
+          if idx == |lookup'| - 2 {
+            assert BT.LookupFollowsChildRefAtLayer(lookup', idx);
+            assert BT.LookupFollowsChildEdgeAtLayer(lookup', idx);
           } else {
-            assert PBS.LookupFollowsChildRefAtLayer(startKey, lookup, idx);
-            assert PBS.LookupFollowsChildRefAtLayer(startKey, lookup1, idx);
+            assert BT.LookupFollowsChildRefAtLayer(lookup, idx);
+            assert BT.LookupFollowsChildRefAtLayer(lookup', idx);
+            assert BT.LookupFollowsChildEdgeAtLayer(lookup, idx);
+            assert BT.LookupFollowsChildEdgeAtLayer(lookup', idx);
           }
         }
 
-        var pivot := node.pivotTable[r+1];
-        var upTo' := 
-          if pivot.Max_Element? then (
-            upTo
+        if |lookup'| == 1 {
+          assert tt' == BT.LookupTranslationTable(lookup', 0, None) by {
+            BT.reveal_LookupTranslationTable();
+          }
+        } else {
+          assert tt == BT.LookupTranslationTable(lookup, 0, None);
+          TranslationTableEquiv(lookup', tt');
+          assert tt' == BT.LookupTranslationTable(lookup', 0, None);
+        }
+
+        var upper := 
+          if pset.None? then (
+              node.pivotTable[r+1]
           ) else (
-            var ub := GetKey(node.pivotTable, r+1);
-            if upTo.Some?
-            then (
-              var k: Key := if lt(upTo.value, ub) then upTo.value else ub;
-              Some(k)
-            ) else (
-              Some(ub)
-            )
+            var (left, right) := TranslatePivotPairInternal(KeyToElement(key), node.pivotTable[r+1], pset.value.prefix, pset.value.newPrefix);
+            right
           );
 
-        assert upTo'.Some? ==> lt(startKey, upTo'.value);
+        var upTo' := 
+          if upper.Max_Element? then upTo 
+          else (
+            var ub : Key := upper.e;
+            if upTo.None? then (
+              Some(ub)
+            ) else (
+              var k: Key := if lt(upTo.value, upper.e) then upTo.value else ub;
+              Some(k)
+            ));
 
-        PBS.reveal_LookupUpperBound();
+        assert upTo'.Some? ==> lt(startKey, upTo'.value);
+        assert tt' == BT.LookupTranslationTable(lookup', 0, None);
+        assert upTo' == BT.LookupUpperBound(lookup', tt') 
+          by { BT.reveal_LookupUpperBound(); }
 
         if node.children.Some? {
           if counter == 0 {
             assert noop(s, s);
           } else {
             lemmaChildInGraph(s, ref, node.children.value[r]);
-            lemmaGetPathResult(s, io, startKey, acc1, lookup1, start, upTo', maxToFind, node.children.value[r], counter - 1);
+            var translate := Translate(node.pivotTable, node.edgeTable, key);
+            var key' := ApplyPrefixSet(translate, key);
+
+            assert translate.Some? ==> IsPrefix(translate.value.prefix, key);
+            assert pset.Some? ==> IsPrefix(pset.value.prefix, key);
+
+            var pset' := ComposePrefixSet(pset, translate);
+            ComposePrefixSetCorrect(pset, translate, pset', startKey, key, key');
+            lemmaGetPathResult(s, io, startKey, key', acc', tt', lookup', start, upTo', pset', maxToFind, node.children.value[r], counter - 1);
           }
         } else {
           var res :=
-            BucketSuccessorLoopModel.GetSuccessorInBucketStack(acc1, maxToFind, start, upTo');
-          SatisfiesSuccBetreeStep(s, io, start, res, acc1, lookup1, maxToFind, startKey, upTo');
+            BucketSuccessorLoopModel.GetSuccessorInBucketStack(acc', tt', maxToFind, start, upTo');
+          SatisfiesSuccBetreeStep(s, io, start, res, acc', tt', lookup', maxToFind, startKey, upTo');
         }
       } else {
         assert noop(s, s);
@@ -317,7 +470,7 @@ module SuccModel {
             betree_next_dop(IBlockCache(s), IBlockCache(s'), IDiskOp(diskOp(io')).bdop))
   {
     reveal_doSucc();
-    PBS.reveal_LookupUpperBound();
+    BT.reveal_LookupUpperBound();
     var startKey := if start.NegativeInf? then [] else start.key;
     lemmaGetPathResult(s, io, startKey, [], [], start, None, maxToFind, BT.G.Root(), 40);
   }
