Impl/BucketIteratorModel.i.dfy
@@ -1,0 +1,422 @@
+// Copyright 2018-2021 VMware, Inc., Microsoft Inc., Carnegie Mellon University, ETH Zurich, and University of Washington
+// SPDX-License-Identifier: BSD-2-Clause
+
+include "../lib/Buckets/BucketsLib.i.dfy"
+include "../lib/Buckets/TranslationLib.i.dfy"
+include "../lib/Base/Sets.i.dfy"
+
+//
+// A mathematical description of bucket iterators for successor query.
+//
+
+module BucketIteratorModel {
+  import opened Options
+  import opened Sets
+  import opened BucketsLib
+  import Keyspace = Lexicographic_Byte_Order
+  import opened ValueMessage
+  import opened Sequences
+  import opened KeyType
+  import opened BucketMaps
+  import opened TranslationLib
+  import MapSeqs
+
+  datatype IteratorOutput = Next(key: Key, msg: Message) | Done
+
+  datatype Iterator = Iterator(
+    pset: Option<PrefixSet>,
+    ghost next: IteratorOutput,
+    ghost idx: int,
+    ghost decreaser: int
+  )
+
+  function SetGte(bucket: BucketMap, key: Key) : set<Key>
+  {
+    set k | k in bucket && Keyspace.lte(key, k)
+  }
+
+  function SuccBucket(bucket: Bucket, pset: Option<PrefixSet>): Bucket
+  requires PreWFBucket(bucket)
+  {
+    if pset.None? then bucket else TranslateBucket(bucket, pset.value.prefix, pset.value.newPrefix)
+  }
+
+  function SuccIdx(bucket: Bucket, pset: Option<PrefixSet>, idx: int): (i: int)
+  requires PreWFBucket(bucket)
+  requires 0 <= idx < |bucket.keys|
+  requires pset.Some? ==> IsPrefix(pset.value.prefix, bucket.keys[idx])
+  ensures 0 <= i < |SuccBucket(bucket, pset).keys|
+  ensures SuccBucket(bucket, pset).keys[i] == ApplyPrefixSet(pset, bucket.keys[idx])
+  {
+    if pset.None? then idx else (
+      var tbucket := TranslateBucketInternal(bucket, pset.value.prefix, pset.value.newPrefix, 0);
+      var i :| 0 <= i < |tbucket.idxs| && tbucket.idxs[i] == idx;
+      i
+    )
+  }
+
+  predicate WFIterNext(bucket: Bucket, it: Iterator)
+  requires PreWFBucket(bucket)
+  requires it.next.Next?
+  {
+    && it.decreaser > 0
+    && 0 <= it.idx < |bucket.keys|
+    && (it.pset.Some? ==> IsPrefix(it.pset.value.prefix, bucket.keys[it.idx]))
+    && it.next.key == ApplyPrefixSet(it.pset, bucket.keys[it.idx])
+    && it.next.msg == bucket.msgs[it.idx]
+  }
+
+  predicate {:opaque} WFIter(bucket: Bucket, it: Iterator)
+  ensures WFIter(bucket, it) ==>
+      && PreWFBucket(bucket)
+      && it.decreaser >= 0
+      && (it.next.Next? && BucketWellMarshalled(bucket) ==> (
+        && it.next.key in SuccBucket(bucket, it.pset).as_map()
+        && it.next.msg == SuccBucket(bucket, it.pset).as_map()[it.next.key]
+      ))
+  {
+    && PreWFBucket(bucket)
+    && it.decreaser >= 0
+    && it.idx >= 0
+    && it.idx + it.decreaser == |bucket.keys|
+    && |bucket.keys| == |bucket.msgs|
+    && (it.next.Next? ==> WFIterNext(bucket, it))
+    && (it.next.Done? ==> it.decreaser == 0)
+    && (it.next.Next? && BucketWellMarshalled(bucket) ==> (
+        && it.next.key in SuccBucket(bucket, it.pset).as_map()
+        && it.next.msg == SuccBucket(bucket, it.pset).as_map()[it.next.key]
+    ))
+  }
+
+  function iterForIndex(bucket: Bucket, pset: Option<PrefixSet>,  idx: int) : (it: Iterator)
+  requires PreWFBucket(bucket)
+  requires 0 <= idx <= |bucket.keys|
+  requires idx < |bucket.keys| && pset.Some? ==> IsPrefix(pset.value.prefix, bucket.keys[idx])
+  ensures WFIter(bucket, it)
+  {
+    reveal WFIter();
+
+    var next := if idx == |bucket.keys| then Done else Next(ApplyPrefixSet(pset, bucket.keys[idx]), bucket.msgs[idx]);
+
+    var it := Iterator(pset, next, idx, |bucket.keys| - idx);
+    assert (it.next.Next? && BucketWellMarshalled(bucket) ==> (
+      var succidx := SuccIdx(bucket, pset, idx);
+      var succbucket := SuccBucket(bucket, pset);
+
+      MapSeqs.MapMapsIndex(succbucket.keys, succbucket.msgs, succidx);
+      && it.next.key in succbucket.as_map()
+      && it.next.msg == succbucket.as_map()[it.next.key]
+    ));
+    it
+  }
+
+  function iterEnd(bucket: Bucket) : (it: Iterator)
+  requires |bucket.keys| == |bucket.msgs|
+  ensures WFIter(bucket, it)
+  {
+    reveal WFIter();
+    Iterator(None, Done, |bucket.keys|, 0)
+  }
+
+  ///// Functions for initializing and manipulating iterators
+
+  // linear search
+  // function iterNextWithPrefix(bucket: Bucket, prefix: Key, idx: int) : (i: int)
+  // requires PreWFBucket(bucket)
+  // requires 0 <= idx <= |bucket.keys|
+  // ensures idx <= i <= |bucket.keys|
+  // ensures i < |bucket.keys| ==> IsPrefix(prefix, bucket.keys[i])
+  // ensures forall j | idx <= j < i :: !IsPrefix(prefix, bucket.keys[j])
+  // decreases |bucket.keys| - idx
+  // {
+  //   if idx < |bucket.keys| && !IsPrefix(prefix, bucket.keys[idx]) then (
+  //     iterNextWithPrefix(bucket, prefix, idx+1)
+  //   ) else (
+  //     idx
+  //   )
+  // }
+
+  function iterNextWithPrefix(bucket: Bucket, prefix: Key, idx: int) : (i: int)
+  requires PreWFBucket(bucket)
+  requires 0 <= idx <= |bucket.keys|
+  ensures idx <= i <= |bucket.keys|
+  ensures i < |bucket.keys| ==> IsPrefix(prefix, bucket.keys[i])
+  ensures BucketWellMarshalled(bucket) ==> forall j | idx <= j < i :: !IsPrefix(prefix, bucket.keys[j])
+  {
+    Keyspace.reveal_IsStrictlySorted();
+    reveal_IsPrefix();
+
+    if idx == |bucket.keys| then (
+      idx
+    ) else if IsPrefix(prefix, bucket.keys[idx]) then (
+      idx
+    ) else if Keyspace.lt(bucket.keys[idx], prefix) then (
+      var i := Keyspace.binarySearchIndexOfFirstKeyGteWithLowerBound(bucket.keys, prefix, idx+1);
+      AllKeysLtPrefix(prefix);
+
+      if i < |bucket.keys| then (
+        if IsPrefix(prefix, bucket.keys[i]) then (
+          i
+        ) else (
+          AllKeysWithPrefixLt(prefix, bucket.keys[i]);
+          |bucket.keys|
+        )
+      ) else (
+        |bucket.keys|
+      )
+    ) else (
+      AllKeysWithPrefixLt(prefix, bucket.keys[idx]);
+      |bucket.keys|
+    )
+  }
+
+  function {:opaque} IterStart(bucket: Bucket, pset: Option<PrefixSet>) : (it' : Iterator)
+  requires WFBucket(bucket)
+  ensures WFIter(bucket, it')
+  ensures it'.pset == pset
+  {
+    reveal WFIter();
+
+    var i := if pset.None? then 0 else iterNextWithPrefix(bucket, pset.value.prefix, 0);
+    iterForIndex(bucket, pset, i)
+  }
+
+  function {:opaque} IterFindFirstGte(bucket: Bucket, pset: Option<PrefixSet>, key: Key) : (it' : Iterator)
+  requires WFBucket(bucket)
+  requires pset.Some? ==> IsPrefix(pset.value.newPrefix, key)
+  ensures WFIter(bucket, it')
+  ensures it'.pset == pset
+  {
+    var key' := ApplyPrefixSet(RevPrefixSet(pset), key);
+    var start := Keyspace.binarySearchIndexOfFirstKeyGte(bucket.keys, key');
+    var i := if pset.None? then start else iterNextWithPrefix(bucket, pset.value.prefix, start);
+    iterForIndex(bucket, pset, i)
+  }
+
+  function {:opaque} IterFindFirstGt(bucket: Bucket, pset: Option<PrefixSet>, key: Key) : (it' : Iterator)
+  requires WFBucket(bucket)
+  requires pset.Some? ==> IsPrefix(pset.value.newPrefix, key)
+  ensures WFIter(bucket, it')
+  ensures it'.pset == pset
+  {
+    reveal WFIter();
+
+    var key' := ApplyPrefixSet(RevPrefixSet(pset), key);
+    var start := Keyspace.binarySearchIndexOfFirstKeyGt(bucket.keys, key');
+    var i := if pset.None? then start else iterNextWithPrefix(bucket, pset.value.prefix, start);
+    iterForIndex(bucket, pset, i)
+  }
+
+  function {:opaque} IterInc(bucket: Bucket, it: Iterator) : (it' : Iterator)
+  requires WFBucket(bucket)
+  requires WFIter(bucket, it)
+  requires it.next.Next?
+  ensures WFIter(bucket, it')
+  ensures it'.pset == it.pset
+  ensures it'.decreaser < it.decreaser
+  {
+    reveal WFIter();
+
+    var i := if it.pset.None? then it.idx+1 else iterNextWithPrefix(bucket, it.pset.value.prefix, it.idx+1);
+    iterForIndex(bucket, it.pset, i)
+  }
+
+  lemma KeyIdx(bucket: Bucket, pset:Option<PrefixSet>, key: Key) returns (i: int)
+  requires PreWFBucket(bucket)
+  requires key in SuccBucket(bucket, pset).as_map()
+  ensures 0 <= i < |bucket.keys|
+  ensures pset.Some? ==> IsPrefix(pset.value.prefix, bucket.keys[i])
+  ensures ApplyPrefixSet(pset, bucket.keys[i]) == key
+  {
+    if pset.None? {
+      i := MapSeqs.GetIndex(bucket.keys, bucket.msgs, key);
+    } else {
+      var tbucket := TranslateBucketInternal(bucket, pset.value.prefix, pset.value.newPrefix, 0);
+      var succidx := MapSeqs.GetIndex(tbucket.b.keys, tbucket.b.msgs, key);
+      i := tbucket.idxs[succidx];
+    }
+  }
+
+  lemma noKeyBetweenIterAndIterInc(bucket: Bucket, it: Iterator, key: Key)
+  requires WFBucket(bucket)
+  requires BucketWellMarshalled(bucket)
+  requires WFIter(bucket, it)
+  requires key in SuccBucket(bucket, it.pset).as_map()
+  requires it.next.Next?
+  ensures IterInc(bucket, it).next.Next? ==>
+      ( Keyspace.lte(key, it.next.key) || Keyspace.lte(IterInc(bucket, it).next.key, key))
+  ensures IterInc(bucket, it).next.Done? ==>
+        Keyspace.lte(key, it.next.key)
+  {
+    reveal WFIter();
+    Keyspace.reveal_IsStrictlySorted();
+    reveal_IterInc();
+
+    var idx := KeyIdx(bucket, it.pset, key);
+    if it.pset.Some? {
+      var itinc := IterInc(bucket, it);
+      assert idx <= it.idx || itinc.idx <= idx;
+      if idx <= it.idx {
+        PrefixLteProperties(it.pset.value.prefix, bucket.keys[idx], bucket.keys[it.idx]);
+        PrefixLteProperties(it.pset.value.newPrefix, key, it.next.key);
+        assert Keyspace.lte(key, it.next.key);
+      } else {
+        PrefixLteProperties(it.pset.value.prefix, bucket.keys[itinc.idx], bucket.keys[idx]);
+        PrefixLteProperties(it.pset.value.newPrefix, itinc.next.key, key);
+        assert Keyspace.lte(itinc.next.key, key);
+      }
+    }   
+  }
+
+  lemma IterIncKeyGreater(bucket: Bucket, it: Iterator)
+  requires WFIter(bucket, it)
+  requires it.next.Next?
+  requires WFBucket(bucket)
+  requires BucketWellMarshalled(bucket)
+  ensures IterInc(bucket, it).next.Next? ==>
+      Keyspace.lt(it.next.key, IterInc(bucket, it).next.key)
+  {
+    reveal WFIter();
+    Keyspace.reveal_IsStrictlySorted();
+    reveal_IterInc();
+
+    var itinc := IterInc(bucket, it);
+    if itinc.next.Next? && it.pset.Some? {
+      PrefixLteProperties(it.pset.value.prefix, bucket.keys[it.idx], bucket.keys[itinc.idx]);
+      PrefixLteProperties(it.pset.value.newPrefix, it.next.key, itinc.next.key);
+    }
+  }
+
+  lemma noKeyBetweenIterFindFirstGte(bucket: Bucket, pset: Option<PrefixSet>, key: Key, key0: Key)
+  requires WFBucket(bucket)
+  requires BucketWellMarshalled(bucket)
+  requires key0 in SuccBucket(bucket, pset).as_map()
+  requires pset.Some? ==> IsPrefix(pset.value.newPrefix, key)
+  ensures IterFindFirstGte(bucket, pset, key).next.Next? ==>
+      (Keyspace.lt(key0, key) || Keyspace.lte(IterFindFirstGte(bucket, pset, key).next.key, key0))
+  ensures IterFindFirstGte(bucket, pset, key).next.Done? ==>
+      (Keyspace.lt(key0, key))
+  {
+    Keyspace.reveal_IsStrictlySorted();
+    reveal_IterFindFirstGte();
+
+    var idx := KeyIdx(bucket, pset, key0);
+    if pset.Some? {
+      var itgte := IterFindFirstGte(bucket, pset, key);
+      if itgte.next.Done? || idx < itgte.idx {
+        var k := ApplyPrefixSet(RevPrefixSet(pset), key);
+        assert Keyspace.lt(bucket.keys[idx], k); // observe
+        PrefixLteProperties(pset.value.prefix, bucket.keys[idx], k);
+        PrefixLteProperties(pset.value.newPrefix, key0, key);
+        assert Keyspace.lt(key0, key);
+      } else {
+        PrefixLteProperties(pset.value.prefix, bucket.keys[itgte.idx], bucket.keys[idx]);
+        PrefixLteProperties(pset.value.newPrefix, itgte.next.key, key0);
+        assert Keyspace.lte(itgte.next.key, key0);
+      }
+    } 
+  }
+
+  lemma IterFindFirstGteKeyGreater(bucket: Bucket, pset: Option<PrefixSet>, key: Key)
+  requires WFBucket(bucket)
+  requires BucketWellMarshalled(bucket)
+  requires pset.Some? ==> IsPrefix(pset.value.newPrefix, key)
+  ensures IterFindFirstGte(bucket, pset, key).next.Next? ==> 
+      Keyspace.lte(key, IterFindFirstGte(bucket, pset, key).next.key)
+  {
+    reveal WFIter();
+    Keyspace.reveal_IsStrictlySorted();
+    reveal_IterFindFirstGte();
+
+    var itgte := IterFindFirstGte(bucket, pset, key);
+    if itgte.next.Next? && pset.Some? {
+      var key' := ApplyPrefixSet(RevPrefixSet(pset), key);
+      PrefixLteProperties(pset.value.prefix, key',  bucket.keys[itgte.idx]);
+      PrefixLteProperties(pset.value.newPrefix, key, itgte.next.key);
+    }
+  }
+
+  lemma noKeyBetweenIterFindFirstGt(bucket: Bucket, pset: Option<PrefixSet>, key: Key, key0: Key)
+  requires WFBucket(bucket)
+  requires BucketWellMarshalled(bucket)
+  requires key0 in SuccBucket(bucket, pset).as_map()
+  requires pset.Some? ==> IsPrefix(pset.value.newPrefix, key)
+  ensures IterFindFirstGt(bucket, pset, key).next.Next? ==>
+      (Keyspace.lte(key0, key) || Keyspace.lte(IterFindFirstGt(bucket, pset, key).next.key, key0))
+  ensures IterFindFirstGt(bucket, pset, key).next.Done? ==>
+      (Keyspace.lte(key0, key))
+  {
+    Keyspace.reveal_IsStrictlySorted();
+    reveal_IterFindFirstGt();
+
+    var idx := KeyIdx(bucket, pset, key0);
+    var itgt := IterFindFirstGt(bucket, pset, key);
+    if pset.Some? {
+      if itgt.next.Done? || idx < itgt.idx {
+        var k := ApplyPrefixSet(RevPrefixSet(pset), key);
+        assert Keyspace.lte(bucket.keys[idx], k); // observe
+        PrefixLteProperties(pset.value.prefix, bucket.keys[idx], k);
+        PrefixLteProperties(pset.value.newPrefix, key0, key);
+        assert Keyspace.lte(key0, key);
+      } else {
+        PrefixLteProperties(pset.value.prefix, bucket.keys[itgt.idx], bucket.keys[idx]);
+        PrefixLteProperties(pset.value.newPrefix, itgt.next.key, key0);
+        assert Keyspace.lte(itgt.next.key, key0);
+      }
+    }
+  }
+
+  lemma IterFindFirstGtKeyGreater(bucket: Bucket, pset: Option<PrefixSet>, key: Key)
+  requires WFBucket(bucket)
+  requires BucketWellMarshalled(bucket)
+  requires pset.Some? ==> IsPrefix(pset.value.newPrefix, key)
+  ensures IterFindFirstGt(bucket, pset, key).next.Next? ==> 
+      Keyspace.lt(key, IterFindFirstGt(bucket, pset, key).next.key)
+  {
+    reveal WFIter();
+    Keyspace.reveal_IsStrictlySorted();
+    reveal_IterFindFirstGt();
+
+    var itgt := IterFindFirstGt(bucket, pset, key);
+    if itgt.next.Next? && pset.Some? {
+      var key' := ApplyPrefixSet(RevPrefixSet(pset), key);
+      assert Keyspace.lt(key', bucket.keys[itgt.idx]); // observe
+      PrefixLteProperties(pset.value.prefix, key', bucket.keys[itgt.idx]);
+      PrefixLteProperties(pset.value.newPrefix, key, itgt.next.key);
+    }
+  }
+
+  lemma noKeyBeforeIterStart(bucket: Bucket, pset: Option<PrefixSet>, key0: Key)
+  requires WFBucket(bucket)
+  requires BucketWellMarshalled(bucket)
+  requires key0 in SuccBucket(bucket, pset).as_map()
+  ensures IterStart(bucket, pset).next.Next?
+  ensures Keyspace.lte(IterStart(bucket, pset).next.key, key0)
+  {
+    Keyspace.reveal_IsStrictlySorted();
+    reveal_IterStart();
+
+    var idx := KeyIdx(bucket, pset, key0);
+    var itstart := IterStart(bucket, pset);
+    if pset.Some? && itstart.idx < idx {
+      PrefixLteProperties(pset.value.prefix, bucket.keys[itstart.idx], bucket.keys[idx]);
+      PrefixLteProperties(pset.value.newPrefix, itstart.next.key, key0);
+    }
+  }
+
+  lemma lemma_NextFromIndex(bucket: Bucket, it: Iterator)
+  requires WFIter(bucket, it)
+  ensures |bucket.keys| == |bucket.msgs|
+  ensures 0 <= it.idx <= |bucket.keys|
+  ensures 0 <= it.idx < |bucket.keys| ==>
+    && it.next.Next?
+    && (it.pset.Some? ==> IsPrefix(it.pset.value.prefix, bucket.keys[it.idx]))
+    && it.next.key == ApplyPrefixSet(it.pset, bucket.keys[it.idx])
+    && it.next.msg == bucket.msgs[it.idx]
+  ensures it.idx == |bucket.keys| ==>
+    && it.next.Done?
+  {
+    reveal WFIter();
+  }
+
+}
