Impl/CloneImpl.i.dfy
@@ -1,0 +1,105 @@
+// Copyright 2018-2021 VMware, Inc., Microsoft Inc., Carnegie Mellon University, ETH Zurich, and University of Washington
+// SPDX-License-Identifier: BSD-2-Clause
+
+include "CloneModel.i.dfy"
+include "FlushPolicyImpl.i.dfy"
+include "DiskOpImpl.i.dfy"
+include "BookkeepingImpl.i.dfy"
+include "MainDiskIOHandler.s.dfy"
+
+module CloneImpl {
+  import CloneModel
+  import IOModel
+  import opened NodeImpl
+  import opened IOImpl
+  import opened BookkeepingImpl
+  import opened MainDiskIOHandler
+  import opened InterpretationDiskOps
+  import opened DiskOpImpl
+  import opened StateBCImpl
+  import opened ViewOp
+  import opened DiskOpModel
+  import opened FlushPolicyImpl
+  import opened BoundedPivotsLib
+  import opened KeyType
+  import opened Bounds
+
+  method doClone(linear inout s: ImplVariables, from: Key, to: Key) returns (success: bool)
+  requires old_s.Inv() && old_s.Ready?
+  requires BT.G.Root() in old_s.I().cache
+  requires |old_s.ephemeralIndirectionTable.I().graph| <= IT.MaxSize() - 1
+  ensures s.Ready?
+  ensures s.W()
+  ensures s.WriteAllocConditions() 
+  ensures LruModel.I(s.lru.Queue()) == s.cache.I().Keys;
+  ensures (s.I(), success) == CloneModel.doClone(old_s.I(), from, to)
+  {
+    CloneModel.reveal_doClone();
+    var root := BT.G.Root();
+    success := true;
+
+    if s.frozenIndirectionTable.lSome? {
+      var b := s.frozenIndirectionTable.value.HasEmptyLoc(root);
+      if b {
+        print "giving up; clone can't run because frozen isn't written";
+        success := false;
+      }
+    }
+
+    if success {
+      var oldroot_pivots, _, oldroot_children := s.cache.GetNodeInfo(root);
+      BookkeepingModel.lemmaChildrenConditionsOfNode(s.I(), root);
+
+      var contains := ComputeContainsAllKeys(oldroot_pivots);
+      if (to != [] && oldroot_children.Some? && contains) {
+        linear var rootopt := s.cache.NodeCloneNewRoot(root, from, to);
+        linear match rootopt {
+          case lNone() => { success := false; }
+          case lSome(node) => {
+            CloneModel.lemmaChildrenConditionsCloneNewRoot(s.I(), s.I().cache[root], from, to);
+            writeBookkeeping(inout s, root, node.children);
+            inout s.cache.Overwrite(root, node);
+            assert (s.I(), success) == CloneModel.doClone(old_s.I(), from, to);
+          }
+        }
+      } else {
+        success := false;
+      }
+    }
+  }
+
+  method clone(linear inout s: ImplVariables, io: DiskIOHandler, from: Key, to: Key) returns (success: bool)
+  requires io.initialized()
+  requires old_s.Inv() && old_s.Ready?
+  modifies io
+  ensures s.WFBCVars()
+  ensures ValidDiskOp(diskOp(IIO(io)))
+  ensures IDiskOp(diskOp(IIO(io))).jdop.NoDiskOp?
+  ensures success ==>
+    BBC.Next(old_s.I(), s.I(), IDiskOp(diskOp(IIO(io))).bdop, AdvanceOp(UI.CloneOp(from, to), true))
+  ensures !success ==>
+    IOModel.betree_next_dop(old_s.I(), s.I(), IDiskOp(diskOp(IIO(io))).bdop)
+  {
+    var indirectionTableSize := s.ephemeralIndirectionTable.GetSize();
+    if (!(indirectionTableSize <= IT.MaxSizeUint64() - 3)) {
+      assert IOModel.noop(old_s.I(), s.I());
+      success := false;
+    } else {
+      var rootLookup := s.cache.InCache(BT.G.Root());
+      if !rootLookup {
+        if s.TotalCacheSize() <= MaxCacheSizeUint64() - 1 {
+          PageInNodeReq(inout s, io, BT.G.Root());
+          success := false;
+        } else {
+          print "insert: root not in cache, but cache is full\n";
+          assert IOModel.noop(old_s.I(), s.I());
+          success := false;
+        }
+      } else {
+        CloneModel.doCloneCorrect(old_s.I(), from, to);
+        success := doClone(inout s, from, to);
+        assert (s.I(), success) == CloneModel.doClone(old_s.I(), from, to);
+      }
+    }
+  }
+}
