Impl/GrowImpl.i.dfy
@@ -57,7 +57,7 @@ module GrowImpl {
     }
 
     if !nop {
-      var oldpivots, oldchildren := s.cache.GetNodeInfo(root);
+      var oldpivots, _, oldchildren := s.cache.GetNodeInfo(root);
       var containsall := ComputeContainsAllKeys(oldpivots);
       if !containsall {
         print "giving up; grow can't run because root node is incorrect";
@@ -78,8 +78,8 @@ module GrowImpl {
             linear var buckets := lseq_alloc(1);
             lseq_give_inout(inout buckets, 0, mutbucket);
 
-            linear var newroot := Node(InitPivotTable(), Some([newref]), buckets);
-            assert newroot.I() == BT.G.Node(InitPivotTable(), Some([newref]), [EmptyBucket()]);
+            linear var newroot := Node(InitPivotTable(), [None], Some([newref]), buckets);
+            assert newroot.I() == BT.G.Node(InitPivotTable(), [None], Some([newref]), [EmptyBucket()]);
             assert s.I().cache[root] == old_s.I().cache[root];
 
             writeBookkeeping(inout s, root, Some([newref]));
