Impl/LeafModel.i.dfy
@@ -39,18 +39,16 @@ module LeafModel {
     ) then (
       s
     ) else (
-      // if data was corrupted before we won't allow access to it after repivot
-      if !BoundedBucketList(node.buckets, node.pivotTable) then (
+      if node.edgeTable[0].Some? then (
         s
-      ) else (
+       ) else (
         var pivot := getMiddleKey(node.buckets[0]);
         var pivots := insert(InitPivotTable(), KeyToElement(pivot), 1);
-
         var buckets' := [
             SplitBucketLeft(node.buckets[0], pivot),
             SplitBucketRight(node.buckets[0], pivot)
         ];
-        var newnode := BT.G.Node(pivots, None, buckets');
+        var newnode := BT.G.Node(pivots, [None, None], None, buckets');
         var s1 := writeBookkeeping(s, ref, None);
         var s' := s1.(cache := s1.cache[ref := newnode]);
         s'
@@ -87,7 +85,7 @@ module LeafModel {
       return;
     }
 
-    if !BoundedBucketList(node.buckets, node.pivotTable) {
+    if node.edgeTable[0].Some? {
       assert noop(s, s);
       return;
     }
@@ -105,7 +103,7 @@ module LeafModel {
 
     //reveal_WFBucket();
 
-    var newnode := BT.G.Node(pivots, None, buckets');
+    var newnode := BT.G.Node(pivots, [None, None], None, buckets');
     var s1 := writeWithNode(s, ref, newnode);
     reveal_writeBookkeeping();
 
@@ -116,6 +114,7 @@ module LeafModel {
     WeightBucketList2(
         SplitBucketLeft(node.buckets[0], pivot),
         SplitBucketRight(node.buckets[0], pivot));*/
+
     PivotBetreeSpecWFNodes.WFApplyRepivot(
         BT.Repivot(ref, node, pivots, pivot));
 
