lib/Lang/LinearSequence.s.dfy
@@ -108,6 +108,7 @@ module {:extern "LinearExtern"} LinearSequence_s {
   method {:extern "LinearExtern", "lseq_length_bound"} lseq_length_bound<A(00)>(shared s:lseq<A>)
     ensures |lseqs_raw(s)| < 0xffff_ffff_ffff_ffff
 
+    // TODO(robj): I think this interface is broken and we should kill it.
   method {:extern "LinearExtern", "TrustedRuntimeSeqResize"} TrustedRuntimeSeqResize<A>(linear s: seq<A>, newlen: uint64)
     returns (linear s2: seq<A>)
     ensures |s2| == newlen as nat
